Test/comp/BranchCoverage.dfy
@@ -1,32 +1,25 @@
 // RUN: %dafny /compile:3 /coverage:- /spillTargetCode:1 /compileTarget:cs BranchCoverage2.cs "%s" > "%t"
 // RUN: %diff "%s.expect" "%t"
 
-method Main() {
-  // we get here 1 time
-  var y := M(5);
-  y := M(y);
-  y := M(y);
+// The Main method is at the end of this file, because that makes it easier to maintain
+// this test file when adding more tests.
 
-  y := N(5);
-  y := N(y);
-  y := N(y);
+// ---------- class constructor ----------
 
-  P(5);
-
-  // do else-if correctly
-  // if-then-else expressions
-  // &&, ||, ==>, <==
-  // if-case
-  // if *
-  // while
-  // match
-  // beginning of functions, methods, including tail recursion?
-  // beginning of forall/exists bodies, set comprehensions, map comprehensions
-  // beginning of labmdas
+class MyClass {
+  constructor () {  // 3 times
+  }
 }
+
+// ---------- routines that are never called ----------
 
 method NeverCalled() {
   // we get here 0 times
+}
+
+function method FunctionNeverCalled(): int {
+  // we get here 0 times
+  75
 }
 
 // ---------- if ----------
@@ -79,4 +72,126 @@ method P(x: int) {
     // we get here 0 times
     y := y + 1;
   }  // implicit else: 1 time
+}
+
+// ---------- if case ----------
+
+method Q(x: int) returns (y: int) {
+  // we get here 3 times
+
+  // the following statement is all ghost, so there are no coverage locations in it
+  if {
+    case x < 100 =>
+    case x < 1000 =>
+      assert x < 1_000_000;
+    case 50 <= x =>
+  }
+
+  if
+  case x < 100 =>
+    // we get here 1 time
+  case x < 1000 =>
+    // we get here 1 time, since the compiler lays down the cases in order
+    return 8;
+  case 50 <= x =>
+    // we get here 1 time
+}
+
+// ---------- while ----------
+
+method R(x: int) returns (y: int) {
+  // we get here 1 time
+  var i: nat := 0;
+  while i < x {
+    // we get here 111 times
+    i := i + 1;
+  }
+
+  while * {
+    // we get here 0 times
+    break;
+  }
+
+  while
+    decreases i
+  {
+    case i % 2 == 0 =>
+      // we get here 56 times
+      if i == 0 {
+        // we get here 1 time
+        break;
+      }  // implicit else: 55 times
+      i := i - 1;
+    case i % 4 == 1 =>
+      // we get here 28 times
+      i := i - 1;
+    case 0 < i =>
+      // we get here 28 times
+      i := i - 1;
+  }
+
+  return 40;
+}
+
+// ---------- top-level if-then-else ----------
+
+function method Fib(n: nat): nat {
+  // we get here 465 times
+  if n < 2 then  // then: 233 times
+    n
+  else if false then  // then: 0 times (else-if is omitted)
+    8
+  else  // else: 232 times
+    Fib(n - 2) + Fib(n - 1)
+}
+
+// ---------- top-level match expression, match statement, and tail recursion ----------
+
+function method {:tailrecursion} Factorial(n: nat): nat {
+  // 11 times
+  match n
+  case 0 => 1  // 1 time
+  case _ => n * Factorial(n - 1)  // 10 times
+}
+
+method {:tailrecursion} ComputeFactorial(n: nat, acc: nat) returns (f: nat)
+  ensures f == Factorial(n) * acc
+{
+  // 11 times
+  match n
+  case 0 =>  // 1 time
+    return acc;
+  case _ =>  // 10 times
+    f := ComputeFactorial(n - 1, acc * n);
+}
+
+// ---------- Main ----------
+
+method Main() {
+  // we get here 1 time
+
+  var mc := new MyClass();
+  mc := new MyClass();
+  mc := new MyClass();
+
+  var y := M(5);
+  y := M(y);
+  y := M(y);
+
+  y := N(5);
+  y := N(y);
+  y := N(y);
+
+  P(5);
+
+  y := Q(50);
+  y := Q(101);
+  y := Q(1010);
+
+  y := R(111);
+
+  y := Fib(12);
+
+  y := Factorial(10);
+  y := ComputeFactorial(10, 1);
 }
